pulse/lib/pulse/lib/Pulse.Lib.Deque.fst
@@ -867,14 +867,12 @@ fn rec is_deque_suffix_nolast_helper
       unfold is_deque_suffix p [hd] prev tail last;
       rewrite each p as tail;
       with v. assert (pts_to tail v);
-      ghost fn pf () :
-        trade_f (pts_to tail ({ v with dnext = last' }))
-          (is_deque_suffix p [hd] prev tail last') =
+      intro (pts_to tail ({ v with dnext = last' }) @==>
+          is_deque_suffix p [hd] prev tail last') = _
       {
         rewrite each tail as p;
         fold (is_deque_suffix p [hd] prev tail last');
       };
-      intro_trade _ _ _ pf;
       rewrite each [hd] as l;
       v;
     }
@@ -889,16 +887,14 @@ fn rec is_deque_suffix_nolast_helper
 
       let v = is_deque_suffix_nolast_helper p' (h2 :: tl2) (Some p) tail last last';
 
-      ghost fn pf () :
-        trade_f
-          (pts_to tail ({ v with dnext = last' }))
-          #(pts_to p vp ** trade (pts_to tail { v with dnext = last' }) (is_deque_suffix p' (h2 :: tl2) (Some p) tail last'))
-          (is_deque_suffix p (hd :: h2 :: tl2) prev tail last') =
+      intro (pts_to tail ({ v with dnext = last' }) @==>
+          is_deque_suffix p (hd :: h2 :: tl2) prev tail last')
+        #(pts_to p vp ** trade (pts_to tail { v with dnext = last' }) (is_deque_suffix p' (h2 :: tl2) (Some p) tail last'))
+        = _
       {
         elim_trade _ _;
         fold (is_deque_suffix p (hd :: h2 :: tl2) prev tail last');
       };
-      intro_trade _ _ _ pf;
 
       rewrite each (hd :: h2 :: tl2) as l;
       v;
