pulse/lib/pulse/lib/class/Pulse.Class.Duplicable.fst
@@ -19,7 +19,7 @@ module Pulse.Class.Duplicable
 
 open Pulse.Lib.Core
 
-instance dup_inv (i : iname) (p : slprop)
+instance duplicable_inv (i : iname) (p : slprop)
   : duplicable (inv i p) = {
   dup_f = (fun () -> dup_inv i p);
 }
