pulse/lib/pulse/lib/class/Pulse.Class.Duplicable.fsti
@@ -31,4 +31,4 @@ class duplicable (p : slprop) = {
 let dup (p : slprop) {| d : duplicable p |} ()
   : stt_ghost unit emp_inames p (fun _ -> p ** p) = d.dup_f ()
 
-instance val dup_inv (i : iname) (p : slprop) : duplicable (inv i p)
+instance val duplicable_inv (i : iname) (p : slprop) : duplicable (inv i p)
