pulse/share/pulse/examples/parallel/Promises.Examples3.fst
@@ -122,10 +122,6 @@ fn proof
 }
 
 
-let cheat_proof (i:iname) ()
-  : pledge_f #[i] (pts_to done #0.5R true) #(inv i inv_p ** pts_to claimed #0.5R false) goal
-  = admit() //proof is atomic, not ghost
-
 // #set-options "--debug SMTQuery"
 
 
@@ -151,7 +147,10 @@ fn setup (_:unit)
   let i = new_invariant inv_p;
   inames_live_inv i inv_p;
   GhostSet.lemma_equal_intro (add_inv emp_inames i) (single i);
-  make_pledge _ _ _ _ (cheat_proof i);
+  make_pledge (add_inv emp_inames i) (pts_to done #0.5R true) goal (inv i inv_p ** pts_to claimed #0.5R false) = _ {
+    //cheating: (proof i) is atomic, not ghost
+    admit()
+  };
 
   i
 }
